Tweaking the binary search tree example

teaching/taltech2018/sol/BinarySearchTree.fst
@@ -142,7 +142,30 @@ and treeptr = ref (option node)
 
 let mtree = treeptr
 
-let rec is_stree (r:mtree) (t:stree) (h:heap) : GTot bool (decreases t) =
+let rec wf (r:mtree) (t:stree) (h:heap) : GTot (option (Set.set nat)) (decreases t) =
+  match t , sel h r with
+  | Leaf         , None    -> Some (Set.empty)
+  | Node t1 n t2 , Some nd -> (
+      match wf nd.left t1 h , n = nd.value , wf nd.right t2 h with
+      | Some s1 , true , Some s2 -> Some (Set.union (Set.singleton (addr_of r)) (Set.union s1 s2))
+      | _ -> None
+    )
+  | _                      -> None
+
+let is_stree r t h = Some? (wf r t h)
+
+(*
+  match t with 
+  | Leaf -> None? (sel h r)
+  | Node t1 n t2 -> 
+      Some? (sel h r) &&
+      (match (sel h r) with
+       | Some nd -> wf_mtree nd.left t1 h &&
+                    n = nd.value &&
+                    wf_mtree nd.right t2 h)
+*)
+
+(*let rec is_stree (r:mtree) (t:stree) (h:heap) : GTot bool (decreases t) =
   match t with 
   | Leaf -> None? (sel h r)
   | Node t1 n t2 -> 
@@ -150,7 +173,7 @@ let rec is_stree (r:mtree) (t:stree) (h:heap) : GTot bool (decreases t) =
       (match (sel h r) with
        | Some nd -> is_stree nd.left t1 h &&
                     n = nd.value &&
-                    is_stree nd.right t2 h)
+                    is_stree nd.right t2 h)*)
 
 let rec search (t:erased stree) (r:mtree) (n:nat) 
   : ST bool (requires (fun h0 -> is_stree r (reveal t) h0))
@@ -172,6 +195,7 @@ let create ()
                                                             is_stree r (reveal t) h1)) =
   hide Leaf , alloc None
 
+(*
 let rec addrs_of_tree (r:mtree) (t:stree) (h:heap{is_stree r t h}) 
   : GTot (Set.set nat) (decreases t) = 
   match t with
@@ -181,6 +205,15 @@ let rec addrs_of_tree (r:mtree) (t:stree) (h:heap{is_stree r t h})
       | Some nd -> Set.union (Set.singleton (addr_of r)) 
                              (Set.union (addrs_of_tree nd.left t1 h) 
                                         (addrs_of_tree nd.right t2 h))
+*)
+
+let lemma_is_stree_node (t1 t2:erased stree) (r r1 r2:mtree) (n:nat) (h:heap)
+  : Lemma (requires (sel h r == Some ({ left=r1; value=n; right=r2}) /\
+                     is_stree r1 (reveal t1) h /\ 
+                     is_stree r2 (reveal t2) h /\ 
+                     sorted (Node (reveal t1) n (reveal t2))))
+          (ensures  (is_stree r (Node (reveal t1) n (reveal t2)) h)) = 
+  ()
 
 let rec insert (t:erased stree) (r:mtree) (n:nat) 
   : ST (erased stree) (requires (fun h0 -> is_stree r (reveal t) h0))
@@ -205,7 +238,11 @@ let rec insert (t:erased stree) (r:mtree) (n:nat)
                             let h' = get () in 
                             assert (is_stree (nd.left) (reveal t1') h');
                             assume (is_stree (nd.right) (reveal t2) h');
-                            admit ();
+                            //assert (Node (reveal t1') nd.value (reveal t2) = stree_insert (reveal t) n);
+                            assert (sorted (Node (reveal t1') nd.value (reveal t2)));
+                            assume (sel h' r == Some ({ left=nd.left; value=nd.value; right=nd.right}));
+                            lemma_is_stree_node t1' t2 r nd.left nd.right nd.value h';
+                            //admit ();
                             hide (Node (reveal t1') nd.value (reveal t2)))
                       else (admit ())
 
